ulib/experimental/Steel.PCMReference.fst
@@ -20,8 +20,33 @@ let split #a #p r v v0 v1 =
   split' r v0 v1
 
 let gather r v0 v1 = as_action (gather_action FStar.Set.empty r v0 v1)
-let witness r fact v _ = as_action (Steel.Memory.witness FStar.Set.empty r fact v ())
-let recall #a #pcm #fact r v = as_action (Steel.Memory.recall #a #pcm #fact FStar.Set.empty r v)
+
+val witness' (#a:Type) (#pcm:pcm a)
+            (r:ref a pcm)
+            (fact:stable_property pcm)
+            (v:erased a)
+            (_:fact_valid_compat fact v)
+  : SteelT unit (pts_to r v)
+                (fun _ -> pts_to r v `star` pure (witnessed r fact))
+
+let witness' r fact v _ = as_action (Steel.Memory.witness FStar.Set.empty r fact v ())
+
+let witness r fact v s = witness' r fact v s; elim_pure (witnessed r fact)
+
+val recall' (#a:Type u#1) (#pcm:pcm a) (#fact:property a)
+           (r:ref a pcm)
+           (v:erased a)
+  : SteelT (v1:erased a{compatible pcm v v1})
+           (pts_to r v `star` pure (witnessed r fact))
+           (fun v1 -> pts_to r v `star` pure (fact v1))
+
+let recall' #a #pcm #fact r v = as_action (Steel.Memory.recall #a #pcm #fact FStar.Set.empty r v)
+
+let recall #a #pcm fact r v =
+  intro_pure (witnessed r fact);
+  let v1 = recall' r v in
+  elim_pure (fact v1);
+  v1
 
 let select_refine #a #p r x f = as_action (Steel.Memory.select_refine Set.empty r x f)
 
